{
 "cells": [
  {
   "cell_type": "markdown",
   "metadata": {},
   "source": [
    "# 2.33\n",
    "\n",
    "We consider the system\n",
    "$$\n",
    "\\frac{d y(t)}{d t} + 2\\,y(t)= x(t),\\quad t\\ge0,\n",
    "$$\n",
    "with zero initial conditions (i.e. initial relaxation: $y(0)=0$).\n",
    "\n",
    "We solve the differential equation by multiplying it by the integrating factor\n",
    "$$\n",
    "\\mu(t)=e^{\\int 2\\,dt}=e^{2t}.\n",
    "$$\n",
    "\n",
    "Multiplying both sides by $e^{2t}$ gives\n",
    "$$\n",
    "e^{2t}\\frac{d y(t)}{d t} + 2e^{2t}y(t) = e^{2t}x(t).\n",
    "$$\n",
    "The left-hand side is the derivative of the product $e^{2t}y(t)$; therefore,\n",
    "$$\n",
    "\\frac{d}{dt}\\Bigl[e^{2t}y(t)\\Bigr] = e^{2t} x(t).\n",
    "$$\n",
    "\n",
    "Integrate both sides from 0 to $t$:\n",
    "$$\n",
    "e^{2t}y(t) = \\int_0^t e^{2\\tau}x(\\tau)\\,d\\tau.\n",
    "$$\n",
    "\n",
    "Thus, the general solution is\n",
    "$$\n",
    "y(t)=e^{-2t}\\int_0^t e^{2\\tau}x(\\tau)\\,d\\tau.\n",
    "$$\n",
    "\n",
    "## (a)\n",
    "\n",
    "### (i) When $x_1(t)= e^{3t}u(t)$\n",
    "\n",
    "Substitute $x_1(\\tau)= e^{3\\tau}$ into the integral:\n",
    "$$\n",
    "y_1(t)= e^{-2t}\\int_0^t e^{2\\tau}e^{3\\tau}\\,d\\tau\n",
    "= e^{-2t}\\int_0^t e^{5\\tau}\\,d\\tau.\n",
    "$$\n",
    "Evaluating the integral,\n",
    "$$\n",
    "\\int_0^t e^{5\\tau}\\,d\\tau = \\frac{e^{5t}-1}{5}.\n",
    "$$\n",
    "Thus,\n",
    "$$\n",
    "y_1(t)= e^{-2t}\\cdot\\frac{e^{5t}-1}{5}\n",
    "=\\frac{1}{5}e^{3t}-\\frac{1}{5}e^{-2t}.\n",
    "$$\n",
    "\n",
    "### (ii) When $x_2(t)= e^{2t}u(t)$\n",
    "\n",
    "Substitute $x_2(\\tau)= e^{2\\tau}$ into the general solution:\n",
    "$$\n",
    "y_2(t)= e^{-2t}\\int_0^t e^{2\\tau}e^{2\\tau}\\,d\\tau\n",
    "= e^{-2t}\\int_0^t e^{4\\tau}\\,d\\tau.\n",
    "$$\n",
    "Evaluating the integral,\n",
    "$$\n",
    "\\int_0^t e^{4\\tau}\\,d\\tau = \\frac{e^{4t}-1}{4}.\n",
    "$$\n",
    "Thus,\n",
    "$$\n",
    "y_2(t)= e^{-2t}\\cdot\\frac{e^{4t}-1}{4}\n",
    "=\\frac{1}{4}e^{2t}-\\frac{1}{4}e^{-2t}.\n",
    "$$\n",
    "\n",
    "### (iii) When \n",
    "$$\n",
    "x_3(t)= \\alpha\\,e^{3t}u(t)+ \\beta\\,e^{2t}u(t),\\quad \\alpha,\\beta\\in\\mathbb{R}\n",
    "$$\n",
    "\n",
    "By linearity, the response is given by\n",
    "$$\n",
    "y_3(t)= e^{-2t}\\int_0^t e^{2\\tau}\\Bigl(\\alpha\\,e^{3\\tau}+\\beta\\,e^{2\\tau}\\Bigr)d\\tau.\n",
    "$$\n",
    "Splitting the integral and using the previous results:\n",
    "$$\n",
    "y_3(t)= \\alpha\\,e^{-2t}\\int_0^t e^{5\\tau}\\,d\\tau + \\beta\\,e^{-2t}\\int_0^t e^{4\\tau}\\,d\\tau,\n",
    "$$\n",
    "which yields\n",
    "$$\n",
    "y_3(t) = \\alpha\\left[\\frac{e^{5t}-1}{5}e^{-2t}\\right] + \\beta\\left[\\frac{e^{4t}-1}{4}e^{-2t}\\right].\n",
    "$$\n",
    "That is,\n",
    "$$\n",
    "y_3(t)= \\alpha\\left(\\frac{1}{5}e^{3t}-\\frac{1}{5}e^{-2t}\\right)\n",
    "+\\beta\\left(\\frac{1}{4}e^{2t}-\\frac{1}{4}e^{-2t}\\right).\n",
    "$$\n",
    "\n",
    "This clearly shows that\n",
    "$$\n",
    "y_3(t)= \\alpha\\, y_1(t)+ \\beta\\, y_2(t),\n",
    "$$\n",
    "which confirms the superposition property and the linearity of the system.\n",
    "\n",
    "## (b)\n",
    "\n",
    "### (i) When $x_1(t)= K\\,e^{2t}\\,u(t)$\n",
    "\n",
    "For $t\\ge0$, substitute $x_1(\\tau)= K\\,e^{2\\tau}$ into the formula:\n",
    "$$\n",
    "y_1(t)= e^{-2t}\\int_0^t e^{2\\tau}\\Bigl[K\\,e^{2\\tau}\\Bigr]d\\tau\n",
    "= K\\,e^{-2t}\\int_0^t e^{4\\tau}\\,d\\tau.\n",
    "$$\n",
    "Evaluate the integral:\n",
    "$$\n",
    "\\int_0^t e^{4\\tau}\\,d\\tau = \\frac{e^{4t}-1}{4}.\n",
    "$$\n",
    "Thus, the output becomes\n",
    "$$\n",
    "y_1(t)= K\\,e^{-2t}\\cdot\\frac{e^{4t}-1}{4} = \\frac{K}{4}\\Bigl(e^{2t}- e^{-2t}\\Bigr).\n",
    "$$\n",
    "Including the unit step for clarity,\n",
    "$$\n",
    "y_1(t)=\\frac{K}{4}\\Bigl(e^{2t}- e^{-2t}\\Bigr) u(t).\n",
    "$$\n",
    "\n",
    "### (ii) When $x_2(t)= K\\,e^{2(t-T)}\\,u(t-T)$\n",
    "\n",
    "Here the input is delayed; note that $x_2(t)=0$ for $t < T$. In the solution formula, when integrating we have\n",
    "$$\n",
    "y_2(t)= e^{-2t}\\int_0^t e^{2\\tau}\\,x_2(\\tau)\\,d\\tau.\n",
    "$$\n",
    "Since $x_2(\\tau)= K\\,e^{2(\\tau-T)}\\,u(\\tau-T)$, the integrand is nonzero only for $\\tau \\ge T$. Hence we can write:\n",
    "$$\n",
    "y_2(t)= e^{-2t}\\int_T^t e^{2\\tau}\\,\\Bigl[K\\,e^{2(\\tau-T)}\\Bigr]d\\tau, \\quad t\\ge T.\n",
    "$$\n",
    "Combine the exponentials:\n",
    "$$\n",
    "e^{2\\tau}\\,e^{2(\\tau-T)} = e^{4\\tau-2T}.\n",
    "$$\n",
    "Then\n",
    "$$\n",
    "y_2(t)= K\\,e^{-2t}\\int_T^t e^{4\\tau-2T}\\,d\\tau = K\\,e^{-2t-2T}\\int_T^t e^{4\\tau}\\,d\\tau.\n",
    "$$\n",
    "Evaluate the integral:\n",
    "$$\n",
    "\\int_T^t e^{4\\tau}\\,d\\tau = \\frac{e^{4t} - e^{4T}}{4}.\n",
    "$$\n",
    "Thus,\n",
    "$$\n",
    "y_2(t)= \\frac{K}{4}\\,e^{-2t-2T}\\Bigl(e^{4t} - e^{4T}\\Bigr)\n",
    "= \\frac{K}{4}\\Bigl(e^{2t-2T} - e^{-2t+2T}\\Bigr).\n",
    "$$\n",
    "Recognize that the expression depends on \\( t-T \\). In fact, we may write\n",
    "$$\n",
    "y_2(t)= \\frac{K}{4}\\Bigl(e^{2(t-T)} - e^{-2(t-T)}\\Bigr)u(t-T).\n",
    "$$\n",
    "\n",
    "#### Verification of Time Invariance\n",
    "\n",
    "From part (i) we found\n",
    "$$\n",
    "y_1(t)= \\frac{K}{4}\\Bigl(e^{2t} - e^{-2t}\\Bigr)u(t).\n",
    "$$\n",
    "Thus, if we replace \\( t \\) by \\( t-T \\) we obtain\n",
    "$$\n",
    "y_1(t-T)= \\frac{K}{4}\\Bigl(e^{2(t-T)} - e^{-2(t-T)}\\Bigr)u(t-T),\n",
    "$$\n",
    "which is exactly the expression we obtained for \\(y_2(t)\\). Therefore,\n",
    "$$\n",
    "y_2(t) = y_1(t-T).\n",
    "$$"
   ]
  }
 ],
 "metadata": {
  "language_info": {
   "name": "python"
  }
 },
 "nbformat": 4,
 "nbformat_minor": 2
}
