{
 "cells": [
  {
   "cell_type": "markdown",
   "metadata": {},
   "source": [
    "# 1(3)\n",
    "\n",
    "We are given the following function values:\n",
    "$$\n",
    "f(1)=0,\\quad f(-1)=-3,\\quad f(2)=4.\n",
    "$$\n",
    "\n",
    "We wish to find the quadratic interpolation polynomial in Newton form using the nodes \n",
    "$$\n",
    "x_0=1,\\quad x_1=-1,\\quad x_2=2.\n",
    "$$\n",
    "\n",
    "The Newton interpolation polynomial is expressed as\n",
    "$$\n",
    "P(x) = f(x_0) + f[x_0,x_1](x-x_0) + f[x_0,x_1,x_2](x-x_0)(x-x_1).\n",
    "$$\n",
    "\n",
    "  $$\n",
    "   f[x_0,x_1] = \\frac{f(x_1)-f(x_0)}{x_1-x_0} = \\frac{-3-0}{-1-1} = \\frac{-3}{-2} = \\frac{3}{2}.\n",
    "  $$\n",
    "\n",
    "  $$\n",
    "   f[x_1,x_2] = \\frac{f(x_2)-f(x_1)}{x_2-x_1} = \\frac{4-(-3)}{2-(-1)} = \\frac{7}{3}.\n",
    "  $$\n",
    "\n",
    "  $$\n",
    "   f[x_0,x_1,x_2] = \\frac{f[x_1,x_2]-f[x_0,x_1]}{x_2-x_0} = \\frac{\\frac{7}{3}-\\frac{3}{2}}{2-1}.\n",
    "  $$\n",
    "   Find a common denominator:\n",
    "  $$\n",
    "   \\frac{7}{3} - \\frac{3}{2} = \\frac{14}{6} - \\frac{9}{6} = \\frac{5}{6}.\n",
    "  $$\n",
    "   Thus,\n",
    "  $$\n",
    "   f[x_0,x_1,x_2] = \\frac{5/6}{1} = \\frac{5}{6}.\n",
    "  $$\n",
    "\n",
    "Plug the values into the Newton form:\n",
    "$$\n",
    "P(x) = 0 + \\frac{3}{2}(x-1) + \\frac{5}{6}(x-1)(x-(-1)).\n",
    "$$\n",
    "Since $x-(-1)=x+1$, we have:\n",
    "$$\n",
    "\\boxed{P(x) = \\frac{3}{2}(x-1) + \\frac{5}{6}(x-1)(x+1).}\n",
    "$$\n",
    "\n",
    "Optionally, expanding the product:\n",
    "$$\n",
    "(x-1)(x+1) = x^2-1,\n",
    "$$\n",
    "so\n",
    "$$\n",
    "P(x)= \\frac{3}{2}(x-1) + \\frac{5}{6}(x^2-1).\n",
    "$$\n",
    "\n",
    "To express $P(x)$ in standard form, combine the terms:\n",
    "$$\n",
    "\\begin{aligned}\n",
    "P(x) &= \\frac{5}{6}x^2 + \\frac{3}{2}x -\\left(\\frac{3}{2} + \\frac{5}{6}\\right) \\\\\n",
    "&= \\frac{5}{6}x^2 + \\frac{3}{2}x - \\frac{9+5}{6} \\\\\n",
    "&= \\frac{5}{6}x^2 + \\frac{3}{2}x - \\frac{14}{6} \\\\\n",
    "&= \\frac{5x^2 + 9x - 14}{6}.\n",
    "\\end{aligned}\n",
    "$$\n",
    "\n",
    "Thus, the quadratic interpolation polynomial in Newton form is:\n",
    "$$\n",
    "\\boxed{P(x) = \\frac{3}{2}(x-1) + \\frac{5}{6}(x-1)(x+1),\\quad \\text{or equivalently, } P(x)=\\frac{5x^2+9x-14}{6}.}\n",
    "$$"
   ]
  },
  {
   "cell_type": "markdown",
   "metadata": {},
   "source": [
    "# 3\n",
    "\n",
    "1. **Rounding Error in the Table Entries**\n",
    "\n",
    "   Since the table has 5 significant digits, the rounding error is bounded by\n",
    "   $$\n",
    "   \\delta \\le 0.5 \\times 10^{-5}\n",
    "   $$\n",
    "   Thus, we have an error of roughly\n",
    "   $$\n",
    "   \\delta \\lesssim 5 \\times 10^{-6}.\n",
    "   $$\n",
    "2. **Linear Interpolation Error**\n",
    "\n",
    "   When using linear interpolation between two adjacent table points $z_i$ and $z_{i+1}$ (with spacing $h = 1'$), the interpolation error for a $C^2$ function $f(z)$ is bounded by\n",
    "   $$\n",
    "   E_{\\text{interp}} \\le \\frac{M}{8}(z_{i+1}-z_i)^2,\n",
    "   $$\n",
    "   where\n",
    "   $$\n",
    "   M = \\max_{z\\in[z_i,\\,z_{i+1}]} |f''(z)|.\n",
    "   $$\n",
    "   \n",
    "   Here $f(z) = \\cos z$. Taking $z$ in radians, the second derivative is\n",
    "   $$\n",
    "   f^{(2)}(z) = -\\cos z\n",
    "   $$\n",
    "   and thus $|f''(z)| \\le 1$.  \n",
    "   \n",
    "   we have\n",
    "   $$\n",
    "   E_{\\text{interp}} \\le \\frac{1}{8}\\left(\\frac{\\pi}{10800}\\right)^2.\n",
    "   $$\n",
    "   \n",
    "   Numerically,\n",
    "   $$\n",
    "   \\left(\\frac{\\pi}{10800}\\right)^2 = \\frac{\\pi^2}{10800^2} \\approx \\frac{9.87}{116640000} \\approx 8.46\\times 10^{-8},\n",
    "   $$\n",
    "   so\n",
    "   $$\n",
    "   E_{\\text{interp}} \\le \\frac{8.46\\times 10^{-8}}{8} \\approx 1.06\\times 10^{-8}.\n",
    "   $$\n",
    "   \n",
    "   This interpolation error is negligible compared to the rounding error.\n",
    "\n",
    "---\n",
    "\n",
    "## Total Error Bound\n",
    "\n",
    "The overall error when using linear interpolation is the sum of the table rounding error and the interpolation error. Since\n",
    "$$\n",
    "E_{\\text{total}} \\lesssim \\delta + E_{\\text{interp}} \\approx 5\\times 10^{-6} + 1.06\\times 10^{-8},\n",
    "$$\n",
    "the total error bound is dominated by the rounding error.\n",
    "\n",
    "Thus, we have\n",
    "$$\n",
    "\\boxed{E_{\\text{total}} \\lesssim 5\\times 10^{-6}.}\n",
    "$$\n"
   ]
  },
  {
   "cell_type": "markdown",
   "metadata": {},
   "source": [
    "# 4(2)\n",
    "\n",
    "We wish to prove that if $x_0,x_1,\\dots,x_n$ are distinct nodes and the Lagrange basis polynomials are given by\n",
    "$$\n",
    "\\ell_j(x)=\\prod_{\\substack{0\\le m\\le n\\\\ m\\neq j}} \\frac{x-x_m}{x_j-x_m},\\quad j=0,1,\\dots,n,\n",
    "$$\n",
    "then for any integer $k$ with $1\\le k\\le n$ the following holds identically:\n",
    "$$\n",
    "\\sum_{j=0}^{n}\\bigl(x_j-x\\bigr)^k\\ell_j(x) \\equiv 0.\n",
    "$$\n",
    "\n",
    "## Proof\n",
    "\n",
    "$$\n",
    "\\begin{aligned}\n",
    "\\sum_{j = 0}^n(x_j - x)^k\\ell_j(x)&\\equiv\n",
    "\\sum_{j = 0}^n\\ell_j(x)\\sum_{m = 0}^k(-1)^mx^mx_j^{k - m}\n",
    "\\end{aligned}\n",
    "$$\n",
    "\n",
    "Since we know,\n",
    "$$\n",
    "\\sum_{i = 0}^nx_i^k\\ell_i(x)\\equiv x^k\n",
    "$$\n",
    "\n",
    "Therefore,\n",
    "\n",
    "$$\n",
    "\\begin{aligned}\n",
    "\\sum_{j = 0}^n(x_j - x)^k\\ell_j(x)&\\equiv\n",
    "\\sum_{m = 0}^k\\sum_{j = 0}^n(-1)^mx^mx_j^{k - m}\\ell_j(x) \\\\ &\\equiv\n",
    "\\sum_{m = 0}^k(-1)^mx^m\\sum_{j = 0}^nx_j^{k - m}\\ell_j(x)\\\\ &\\equiv\n",
    "\\sum_{m = 0}^k (-1)^mx^mx^{k-m} \\\\ &\\equiv \n",
    "(x - x)^k \\\\ &\\equiv \n",
    "0\n",
    "\\end{aligned}\n",
    "$$"
   ]
  },
  {
   "cell_type": "markdown",
   "metadata": {},
   "source": [
    "# 6\n",
    "\n",
    "We wish to approximate $f(x)=e^x$ on the interval\n",
    "$$\n",
    "-4 \\le x \\le 4,\n",
    "$$\n",
    "by quadratic interpolation using an equidistant function table. We require that the truncation (interpolation) error be no more than\n",
    "$$\n",
    "10^{-6}.\n",
    "$$\n",
    "\n",
    "## Step 1. Error Formula for Quadratic Interpolation\n",
    "\n",
    "For quadratic interpolation (i.e. interpolation by a polynomial of degree 2) on three nodes $x_0, x_1, x_2$, the interpolation error at any point $x$ in $[x_0, x_2]$ is given by\n",
    "$$\n",
    "R(x)=\\frac{f^{(3)}(\\xi)}{3!}(x-x_0)(x-x_1)(x-x_2),\n",
    "$$\n",
    "for some $\\xi$ in the interval. In our case, the nodes are equally spaced with step size $h$.\n",
    "\n",
    "## Step 2. Maximum Error over a Subinterval\n",
    "\n",
    "Let the three successive nodes be\n",
    "$$\n",
    "x_0,\\quad x_1=x_0+h,\\quad x_2=x_0+2h.\n",
    "$$\n",
    "Define a shifted variable\n",
    "$$\n",
    "t=x-x_0,\\quad\\text{with } t\\in[0,2h].\n",
    "$$\n",
    "Then the error becomes\n",
    "$$\n",
    "R(t)=\\frac{f^{(3)}(\\xi)}{6}\\,t\\,(t-h)\\,(t-2h).\n",
    "$$\n",
    "\n",
    "We wish to bound the maximum of\n",
    "$$\n",
    "|P(t)|=|t\\,(t-h)\\,(t-2h)|\n",
    "$$\n",
    "for $t\\in[0,2h]$. It can be shown (by finding the critical points) that the maximum absolute value is attained at\n",
    "$$\n",
    "t = h\\Bigl(1- \\frac{1}{\\sqrt{3}}\\Bigr),\n",
    "$$\n",
    "so\n",
    "$$\n",
    "\\max_{t\\in[0,2h]}|t\\,(t-h)\\,(t-2h)| = \\frac{2h^3}{3\\sqrt{3}}.\n",
    "$$\n",
    "\n",
    "Thus the maximum interpolation error over any subinterval is bounded by\n",
    "$$\n",
    "|R(x)| \\le \\frac{M_3}{6}\\cdot \\frac{2h^3}{3\\sqrt{3}} = \\frac{M_3 \\, h^3}{9\\sqrt{3}},\n",
    "$$\n",
    "where\n",
    "$$\n",
    "M_3=\\max_{x\\in[-4,4]}|f^{(3)}(x)|.\n",
    "$$\n",
    "\n",
    "## Step 3. Estimating $M_3$ for $f(x)=e^x$\n",
    "\n",
    "Since\n",
    "$$\n",
    "f(x)=e^x,\\quad f^{(3)}(x)=e^x,\n",
    "$$\n",
    "we have\n",
    "$$\n",
    "|f^{(3)}(x)|= e^x.\n",
    "$$\n",
    "On the interval $[-4,4]$ the maximum occurs at $x=4$ so that\n",
    "$$\n",
    "M_3 = e^4.\n",
    "$$\n",
    "\n",
    "## Step 4. Imposing the Error Tolerance\n",
    "\n",
    "We require\n",
    "$$\n",
    "\\frac{e^4\\, h^3}{9\\sqrt{3}} \\le 10^{-6}.\n",
    "$$\n",
    "Solving for $h$, we have\n",
    "$$\n",
    "h^3 \\le \\frac{9\\sqrt{3}\\,10^{-6}}{e^4}.\n",
    "$$\n",
    "Taking cube roots:\n",
    "$$\n",
    "h \\le \\left(\\frac{9\\sqrt{3}\\,10^{-6}}{e^4}\\right)^{\\frac{1}{3}}.\n",
    "$$\n",
    "\n",
    "## Step 5. Evaluating the Expression\n",
    "\n",
    "Using the approximate value $e^4\\approx 54.598$ and $\\sqrt{3}\\approx 1.732$, we have:\n",
    "$$\n",
    "9\\sqrt{3}\\approx 9\\times1.732\\approx 15.588,\n",
    "$$\n",
    "so that\n",
    "$$\n",
    "\\frac{9\\sqrt{3}\\,10^{-6}}{e^4} \\approx \\frac{15.588\\times10^{-6}}{54.598} \\approx 2.853\\times10^{-7}.\n",
    "$$\n",
    "Taking the cube root,\n",
    "$$\n",
    "h\\le (2.853\\times10^{-7})^{1/3}\\approx 6.56\\times10^{-3}.\n",
    "$$\n",
    "\n",
    "## Final Answer\n",
    "\n",
    "To keep the quadratic interpolation truncation error below $10^{-6}$, the step size $h$ for the equidistant function table should be chosen approximately as\n",
    "$$\n",
    "\\boxed{h\\approx6.6\\times10^{-3}.}\n",
    "$$"
   ]
  },
  {
   "cell_type": "markdown",
   "metadata": {},
   "source": [
    "# 7\n",
    "\n",
    "We wish to prove the following two properties of the divided differences.\n",
    "\n",
    "---\n",
    "\n",
    "## Property (1)\n",
    "**Statement:**  \n",
    "If\n",
    "$$\n",
    "F(x)= c\\, f(x),\n",
    "$$\n",
    "then\n",
    "$$\n",
    "F[x_0,x_1,\\dots,x_n] = c\\,f[x_0,x_1,\\dots,x_n].\n",
    "$$\n",
    "\n",
    "**Proof:**  \n",
    "We proceed by induction on $n$.\n",
    "\n",
    "- **Base Case ($n=0$)**:  \n",
    "  The zeroth divided difference is just the function value evaluated at the node:\n",
    "  $$\n",
    "  F[x_0] = F(x_0) = c\\, f(x_0) = c\\, f[x_0].\n",
    "  $$\n",
    "  Thus, the property holds for $n=0$.\n",
    "\n",
    "- **Inductive Step:**  \n",
    "  Assume the property is true for all orders less than $n$. For $n\\ge 1$, by the definition of divided differences (for distinct nodes),\n",
    "  $$\n",
    "  F[x_0,x_1,\\dots,x_n] = \\frac{F[x_1,x_2,\\dots,x_n] - F[x_0,x_1,\\dots,x_{n-1}]}{x_n - x_0}.\n",
    "  $$\n",
    "  By the induction hypothesis, we have:\n",
    "  $$\n",
    "  F[x_1,x_2,\\dots,x_n] = c \\, f[x_1,x_2,\\dots,x_n] \\quad\\text{and}\\quad F[x_0,x_1,\\dots,x_{n-1}] = c\\, f[x_0,x_1,\\dots,x_{n-1}].\n",
    "  $$\n",
    "  Thus,\n",
    "  $$\n",
    "  F[x_0,x_1,\\dots,x_n] = \\frac{ c\\, f[x_1,x_2,\\dots,x_n] - c\\, f[x_0,x_1,\\dots,x_{n-1}]}{x_n-x_0} = c\\, \\frac{f[x_1,x_2,\\dots,x_n]- f[x_0,x_1,\\dots,x_{n-1}]}{x_n-x_0}.\n",
    "  $$\n",
    "  By definition, the last factor is $f[x_0,x_1,\\dots,x_n]$. Hence,\n",
    "  $$\n",
    "  F[x_0,x_1,\\dots,x_n] = c\\,f[x_0,x_1,\\dots,x_n].\n",
    "  $$\n",
    "\n",
    "This completes the proof of Property (1).\n",
    "\n",
    "---\n",
    "\n",
    "## Property (2)\n",
    "**Statement:**  \n",
    "If\n",
    "$$\n",
    "F(x) = f(x)+g(x),\n",
    "$$\n",
    "then\n",
    "$$\n",
    "F[x_0,x_1,\\dots,x_n]= f[x_0,x_1,\\dots,x_n]+g[x_0,x_1,\\dots,x_n].\n",
    "$$\n",
    "\n",
    "**Proof:**  \n",
    "Again, we use induction on $n$.\n",
    "\n",
    "- **Base Case ($n=0$)**:  \n",
    "  $$\n",
    "  F[x_0] = F(x_0)= f(x_0)+g(x_0)= f[x_0]+g[x_0].\n",
    "  $$\n",
    "  Therefore, the property holds for $n=0$.\n",
    "\n",
    "- **Inductive Step:**  \n",
    "  Assume the result is true for orders less than $n$. For $n\\ge1$, by the definition of divided differences,\n",
    "  $$\n",
    "  F[x_0,x_1,\\dots,x_n] = \\frac{F[x_1,x_2,\\dots,x_n]-F[x_0,x_1,\\dots,x_{n-1}]}{x_n - x_0}.\n",
    "  $$\n",
    "  Using the induction hypothesis,\n",
    "  $$\n",
    "  F[x_1,x_2,\\dots,x_n] = f[x_1,x_2,\\dots,x_n] + g[x_1,x_2,\\dots,x_n],\n",
    "  $$\n",
    "  and\n",
    "  $$\n",
    "  F[x_0,x_1,\\dots,x_{n-1}] = f[x_0,x_1,\\dots,x_{n-1}] + g[x_0,x_1,\\dots,x_{n-1}].\n",
    "  $$\n",
    "  Substituting these into the formula,\n",
    "  $$\n",
    "  \\begin{aligned}\n",
    "  F[x_0,x_1,\\dots,x_n] &= \\frac{\\Bigl(f[x_1,x_2,\\dots,x_n] + g[x_1,x_2,\\dots,x_n]\\Bigr) - \\Bigl(f[x_0,x_1,\\dots,x_{n-1}] + g[x_0,x_1,\\dots,x_{n-1}]\\Bigr)}{x_n-x_0} \\\\\n",
    "  &= \\frac{f[x_1,x_2,\\dots,x_n] - f[x_0,x_1,\\dots,x_{n-1}]}{x_n-x_0} + \\frac{g[x_1,x_2,\\dots,x_n] - g[x_0,x_1,\\dots,x_{n-1}]}{x_n-x_0} \\\\\n",
    "  &= f[x_0,x_1,\\dots,x_n] + g[x_0,x_1,\\dots,x_n].\n",
    "  \\end{aligned}\n",
    "  $$\n",
    "\n",
    "This completes the proof of Property (2)."
   ]
  },
  {
   "cell_type": "markdown",
   "metadata": {},
   "source": [
    "# 8\n",
    "\n",
    "已知\n",
    "$$\n",
    "f(x)=x^7+x^4+3x+1,\n",
    "$$\n",
    "\n",
    "求\n",
    "\n",
    "$$\n",
    "f[2^0,2^1,\\dots,2^7] \\quad \\text{and} \\quad f[2^0,2^1,\\dots,2^8].\n",
    "$$\n",
    "\n",
    "## Answer\n",
    "\n",
    "根据 n 阶分差定义我们有\n",
    "\n",
    "$$\n",
    "f[x_0, x_1, \\cdots, x_n]=\\frac{f^{(n)}(\\xi)}{n!}\n",
    "$$\n",
    "\n",
    "其中 $\\xi \\in [x_0, x_n]$\n",
    "\n",
    "对于 $f(x)=x^7+x^4+3x+1$\n",
    "\n",
    "1. **$2^0,2^1,\\dots,2^7$:**\n",
    "  7 阶导为 $7!$ 故\n",
    "  $$\n",
    "   f[2^0,2^1,\\dots,2^7] = 1.\n",
    "  $$\n",
    "\n",
    "1. **$2^0,2^1,\\dots,2^8$:**\n",
    "  8 阶导为 $0$ 故\n",
    "  $$\n",
    "   f[2^0,2^1,\\dots,2^8] = 0.\n",
    "  $$\n",
    "\n",
    "因此\n",
    "\n",
    "$$\n",
    "\\boxed{f[2^0,2^1,\\dots,2^7] = 1 \\quad\\text{and}\\quad f[2^0,2^1,\\dots,2^8] = 0.}\n",
    "$$"
   ]
  },
  {
   "cell_type": "markdown",
   "metadata": {},
   "source": [
    "# 9\n",
    "\n",
    "证明\n",
    "$$\n",
    "\\Delta\\bigl(f_k g_k\\bigr) = f_k\\,\\Delta g_k + g_{k+1}\\,\\Delta f_k.\n",
    "$$\n",
    "\n",
    "## Proof\n",
    "根据差分的定义我们有\n",
    "   $$\n",
    "   \\Delta\\bigl(f_k g_k\\bigr) = f_{k+1}g_{k+1} - f_k g_k.\n",
    "   $$\n",
    "\n",
    "故\n",
    "   $$\n",
    "   f_{k+1}g_{k+1} - f_kg_k = \\Bigl[f_{k+1}g_{k+1} - f_k g_{k+1}\\Bigr] + \\Bigl[f_k g_{k+1} - f_k g_k\\Bigr].\n",
    "   $$\n",
    "\n",
    "   $$\n",
    "   f_{k+1}g_{k+1} - f_kg_{k+1} = g_{k+1}\\bigl(f_{k+1} - f_k\\bigr) = g_{k+1}\\,\\Delta f_k,\n",
    "   $$\n",
    "\n",
    "   $$\n",
    "   f_k g_{k+1} - f_k g_k = f_k\\bigl(g_{k+1} - g_k\\bigr) = f_k\\,\\Delta g_k.\n",
    "   $$\n",
    "\n",
    "   $$\n",
    "   \\Delta\\bigl(f_k g_k\\bigr) = g_{k+1}\\,\\Delta f_k + f_k\\,\\Delta g_k,\n",
    "   $$\n",
    "因此\n",
    "   $$\n",
    "   \\boxed{\\Delta\\bigl(f_k g_k\\bigr) = f_k\\,\\Delta g_k + g_{k+1}\\,\\Delta f_k.}\n",
    "   $$\n",
    "\n",
    "原式得证。"
   ]
  },
  {
   "cell_type": "markdown",
   "metadata": {},
   "source": [
    "# 10\n",
    "\n",
    "We want to prove the following identity:\n",
    "$$\n",
    "\\sum_{k = 0}^{n - 1}f_k\\Delta g_k = f_n g_n - f_0 g_0 - \\sum_{k = 0}^{n - 1}g_{k + 1}\\Delta f_k,\n",
    "$$\n",
    "where the forward difference operator is defined by\n",
    "$$\n",
    "\\Delta f_k=f_{k+1}-f_k\\quad \\text{and}\\quad \\Delta g_k=g_{k+1}-g_k.\n",
    "$$\n",
    "**Proof:**\n",
    "\n",
    "1. Write the telescoping sum:\n",
    "   $$\n",
    "   f_n g_n - f_0 g_0 = \\sum_{k=0}^{n-1}\\Bigl( f_{k+1}g_{k+1} - f_k g_k \\Bigr).\n",
    "   $$\n",
    "\n",
    "2. Use the product rule for finite differences. Recall that (as proved in a previous exercise)\n",
    "   $$\n",
    "   \\Delta(f_k g_k) = f_k\\,\\Delta g_k + g_{k+1}\\,\\Delta f_k.\n",
    "   $$\n",
    "   Hence, for each $k$,\n",
    "   $$\n",
    "   f_{k+1}g_{k+1} - f_k g_k = f_k\\Delta g_k + g_{k+1}\\Delta f_k.\n",
    "   $$\n",
    "\n",
    "3. Substitute the above into the telescoping sum:\n",
    "   $$\n",
    "   f_n g_n - f_0 g_0 = \\sum_{k=0}^{n-1}\\Bigl( f_k\\Delta g_k + g_{k+1}\\Delta f_k\\Bigr)\n",
    "   = \\sum_{k=0}^{n-1}f_k\\Delta g_k + \\sum_{k=0}^{n-1} g_{k+1}\\Delta f_k.\n",
    "   $$\n",
    "\n",
    "4. Rearranging the result gives:\n",
    "   $$\n",
    "   \\sum_{k=0}^{n-1}f_k\\Delta g_k = f_n g_n - f_0 g_0 - \\sum_{k=0}^{n-1} g_{k+1}\\Delta f_k.\n",
    "   $$\n",
    "\n",
    "This completes the proof."
   ]
  },
  {
   "cell_type": "markdown",
   "metadata": {},
   "source": [
    "# 11\n",
    "\n",
    "Prove that\n",
    "\n",
    "$$\n",
    "\\sum_{j = 0}^{n - 1} \\Delta^2 y_j = \\Delta y_n - \\Delta y_0\n",
    "$$\n",
    "\n",
    "**Proof:**\n",
    "\n",
    "Write the telescoping sum\n",
    "\n",
    "$$\n",
    "\\Delta y_n - \\Delta y_0 = \\sum_{j = 0}^{n - 1}\\Delta y_{j + 1} - \\Delta y_j = \\sum_{j = 0}^{n - 1}\\Delta^2y_j\n",
    "$$\n",
    "\n",
    "This completes the proof."
   ]
  },
  {
   "cell_type": "markdown",
   "metadata": {},
   "source": [
    "# 12\n",
    "\n",
    "We are given a polynomial\n",
    "$$\n",
    "f(x)=\\sum_{i=0}^n a_i x^i = a_n\\,(x-x_1)(x-x_2)\\cdots (x-x_n)\n",
    "$$\n",
    "with $n$ distinct real roots $x_1, x_2, \\dots, x_n$. We wish to prove that\n",
    "$$\n",
    "\\sum_{j=1}^n\\frac{x_j^k}{f'(x_j)}=\\begin{cases}0,&0\\le k\\le n-2,\\\\[1mm]\\displaystyle a_n^{-1},& k=n-1.\\end{cases}\n",
    "$$\n",
    "\n",
    "A common strategy is to relate the fractions $\\frac{x_j^k}{f'(x_j)}$ to the partial fractions expansion of a rational function. In particular, note that for any integer (with $\\le k \\le n-1$) the rational function\n",
    "$$\n",
    "\\frac{x^k}{f(x)}\n",
    "$$\n",
    "can be written in the partial-fractions form (its poles are simple at $x_1,\\dots,x_n$):\n",
    "$$\n",
    "\\frac{x^k}{f(x)} = \\sum_{j=1}^{n}\\frac{A_j}{x-x_j},\\quad \\text{with } A_j = \\lim_{x\\to x_j} (x-x_j)\\frac{x^k}{f(x)} = \\frac{x_j^k}{f'(x_j)}.\n",
    "$$\n",
    "Thus,\n",
    "$$\n",
    "\\frac{x^k}{f(x)} = \\sum_{j=1}^n\\frac{x_j^k}{f'(x_j)}\\cdot\\frac{1}{x-x_j}.\n",
    "$$\n",
    "\n",
    "Now, let us compare the asymptotic behavior as $x\\to\\infty$.\n",
    "\n",
    "## Asymptotic Expansion\n",
    "\n",
    "Since\n",
    "$$\n",
    "f(x) = a_nx^n + \\text{(lower order terms)},\n",
    "$$\n",
    "we have for large $x$\n",
    "$$\n",
    "\\frac{x^k}{f(x)} = \\frac{x^k}{a_nx^n}\\Bigl(1+O(1/x)\\Bigr)=\\frac{1}{a_n}\\,x^{k-n}\\Bigl(1+O(1/x)\\Bigr).\n",
    "$$\n",
    "\n",
    "On the other hand, using the expansion of each term in the partial-fractions expansion, for large $x$\n",
    "$$\n",
    "\\frac{1}{x-x_j} = \\frac{1}{x}\\left(1+\\frac{x_j}{x}+\\frac{x_j^2}{x^2}+\\cdots\\right).\n",
    "$$\n",
    "Thus,\n",
    "$$\n",
    "\\sum_{j=1}^n\\frac{x_j^k}{f'(x_j)}\\frac{1}{x-x_j} \n",
    "=\\frac{1}{x}\\sum_{j=1}^n\\frac{x_j^k}{f'(x_j)} \\left[1+\\frac{x_j}{x}+\\frac{x_j^2}{x^2}+\\cdots\\right].\n",
    "$$\n",
    "Collecting the first-order term (i.e. the term proportional to $1/x$), we have\n",
    "$$\n",
    "\\frac{1}{x}\\sum_{j=1}^n\\frac{x_j^k}{f'(x_j)} + \\cdots.\n",
    "$$\n",
    "\n",
    "## Case 1: $\\le k\\le n-2$\n",
    "\n",
    "In this case, the exponent in the asymptotic expansion of the left-hand side is\n",
    "$$\n",
    "x^{k-n},\\quad \\text{with } k-n\\le -2,\n",
    "$$\n",
    "so the left-hand side decays like $1/x^2$(or faster). Thus, there is no \\$/x\\$term in its expansion. Equating the $1/x$ coefficients on both sides yields\n",
    "$$\n",
    "\\sum_{j=1}^n\\frac{x_j^k}{f'(x_j)}=0.\n",
    "$$\n",
    "\n",
    "## Case 2: $=n-1$\n",
    "\n",
    "For $=n-1$, the left-hand side behaves as\n",
    "$$\n",
    "\\frac{x^{n-1}}{f(x)} \\sim \\frac{1}{a_n}\\,\\frac{1}{x},\n",
    "$$\n",
    "so the coefficient of $1/x$ is $1/a_n$ On the other hand, the contribution in the partial-fractions expansion is exactly\n",
    "$$\n",
    "\\frac{1}{x}\\sum_{j=1}^n\\frac{x_j^{n-1}}{f'(x_j)} + \\cdots.\n",
    "$$\n",
    "Equating the two $1/x$ coefficients gives\n",
    "$$\n",
    "\\sum_{j=1}^n\\frac{x_j^{n-1}}{f'(x_j)} = \\frac{1}{a_n}.\n",
    "$$\n",
    "\n",
    "## Conclusion\n",
    "\n",
    "We have shown that\n",
    "$$\n",
    "\\sum_{j=1}^n\\frac{x_j^k}{f'(x_j)}=\\begin{cases}0,&0\\le k\\le n-2,\\\\[1mm]\\displaystyle \\frac{1}{a_n},& k=n-1,\n",
    "\\end{cases}\n",
    "$$\n",
    "which is the desired result.\n",
    "\n",
    "$$\n",
    "\\boxed{\\sum_{j = 1}^n\\frac{x_j^k}{f'(x_j)} = \\begin{cases}\n",
    "0, & 0\\le k \\le n - 2, \\\\\n",
    "a_n^{-1}, & k = n - 1.\n",
    "\\end{cases}}\n",
    "$$"
   ]
  },
  {
   "cell_type": "markdown",
   "metadata": {},
   "source": [
    "# 13\n",
    "\n",
    "We wish to find a polynomial $P(x)$ of degree at most 3 such that\n",
    "$$\n",
    "\\begin{aligned}\n",
    "P(x_0) &= f(x_0), \\\\\n",
    "P'(x_0) &= f'(x_0), \\\\\n",
    "P''(x_0) &= f''(x_0), \\\\\n",
    "P(x_1) &= f(x_1).\n",
    "\\end{aligned}\n",
    "$$\n",
    "\n",
    "Write\n",
    "$$\n",
    "P(x) = a_0 + a_1 (x-x_0) + a_2 (x-x_0)^2 + a_3 (x-x_0)^3.\n",
    "$$\n",
    "Then\n",
    "$$\n",
    "\\begin{aligned}\n",
    "P(x_0) &= a_0,\\\\[1mm]\n",
    "P'(x) &= a_1 + 2a_2 (x-x_0) + 3a_3 (x-x_0)^2,\\quad \\text{so}\\quad P'(x_0)=a_1,\\\\[1mm]\n",
    "P''(x) &= 2a_2 + 6a_3 (x-x_0),\\quad \\text{so}\\quad P''(x_0)=2a_2.\n",
    "\\end{aligned}\n",
    "$$\n",
    "\n",
    "From the conditions,\n",
    "$$\n",
    "\\begin{aligned}\n",
    "a_0 &= f(x_0),\\\\[1mm]\n",
    "a_1 &= f'(x_0),\\\\[1mm]\n",
    "2a_2 &= f''(x_0) \\quad \\Longrightarrow \\quad a_2 = \\frac{f''(x_0)}{2}.\n",
    "\\end{aligned}\n",
    "$$\n",
    "\n",
    "We require\n",
    "$$\n",
    "P(x_1)= f(x_1).\n",
    "$$\n",
    "Since\n",
    "$$\n",
    "P(x_1) = a_0 + a_1 (x_1-x_0) + a_2 (x_1-x_0)^2 + a_3 (x_1-x_0)^3,\n",
    "$$\n",
    "substitute the expressions for $a_0, a_1, a_2$:\n",
    "$$\n",
    "f(x_0) + f'(x_0)(x_1-x_0) + \\frac{f''(x_0)}{2}(x_1-x_0)^2 + a_3 (x_1-x_0)^3 = f(x_1).\n",
    "$$\n",
    "Solve for $a_3$:\n",
    "$$\n",
    "a_3 = \\frac{f(x_1)- f(x_0) - f'(x_0)(x_1-x_0) - \\frac{f''(x_0)}{2}(x_1-x_0)^2}{(x_1-x_0)^3}.\n",
    "$$\n",
    "\n",
    "## Final Form\n",
    "\n",
    "Thus, the desired polynomial is\n",
    "$$\n",
    "\\boxed{\n",
    "f(x_0) + f'(x_0)(x-x_0) + \\frac{f''(x_0)}{2}(x-x_0)^2 + \\frac{f(x_1)- f(x_0) - f'(x_0)(x_1-x_0) - \\frac{f''(x_0)}{2}(x_1-x_0)^2}{(x_1-x_0)^3}(x-x_0)^3.\n",
    "}\n",
    "$$\n",
    "\n",
    "This is the unique polynomial of degree at most 3 that satisfies the given interpolation and derivative conditions."
   ]
  }
 ],
 "metadata": {
  "language_info": {
   "name": "python"
  }
 },
 "nbformat": 4,
 "nbformat_minor": 2
}
