### 18. 解：

$$
f(x)=
\begin{cases}
    \frac{x}{\sigma^2}e^{-\frac{x^2}{2\sigma^2}} & x > 0 \\
    0 & x \leq 0
\end{cases}
$$

其中，$\sigma > 0$

故，

$$
\begin{aligned}
    E(X) &= \int_{-\infty}^{\infty} xf(x)dx \\
    &=\int_{0}^\infty \frac{x^2}{\sigma^2}e^{-\frac{x^2}{2\sigma^2}} dx \\
    &= \int_0^\infty -x de^{-\frac{x^2}{2\sigma ^ 2}}\\
    &= -xe^{-\frac{x^2}{2\sigma^2}}\Big |^{\infty}_{0}+\int_{0}^\infty e^{-\frac{x^2}{2\sigma^2}}dx \\
    &= 0+\sqrt {2\pi}\sigma \int_0^\infty \frac{1}{\sqrt {2\pi}\sigma}e^{-\frac{x^2}{2\sigma^2}}dx\\
    &= \sqrt {\frac{\pi}{2}}\sigma\\
    D(X)&=E(X^2)-E^2(X) \\
    &= \int_0^\infty \frac{x^3}{\sigma^2}e^{-\frac{x^2}{2\sigma^2}}dx-\frac{\pi\sigma^2}{2} \\
    &= \int_0^\infty -x^2de^{-\frac{x^2}{2\sigma^2}}-\frac{\pi\sigma^2}{2}\\
    &= -x^2e^{-\frac{x^2}{2\sigma^2}}\Big |_0^\infty+\int_0^\infty e^{-\frac{x^2}{2\sigma^2}}dx^2-\frac{\pi\sigma^2}{2}\\
    &= 0+(-2\sigma^2e^{-\frac{x^2}{2\sigma^2}})\Big|_0^\infty -\frac{\pi\sigma^2}{2}\\
    &= \sigma^2(2-\frac{\pi}{2})
\end{aligned}
$$