### 10. 解：

#### (1)

令 \( \varsigma^2 = c\sum\limits_{i=1}^{n-1}(X_{i + 1} - X_i)^2 \)

\[
\begin{aligned}
    E(\varsigma^2)&=cE[\sum\limits_{i = 1}^{n - 1}(X_{i + 1} - X_i)^2] = c\sum\limits_{i = 1}^{n - 1}E(X_{i + 1}^2-2X_{i+1}X_i+X_i^2)\\
    &= c\sum\limits_{i=1}^{n-1}(D(X_{i+1})+[E(X_{i+1})]^2-2E(X_{i+1})E(X_i)+D(X_i)+[E(X_{i+1})]^2)\\
    &= c(n-1)(\sigma^2+\mu^2-2\mu^2+\sigma^2+\mu^2)=\sigma^2
\end{aligned}
\]

故有，

\[
c=\frac{1}{2(n-1)}    
\]

#### (2)

\[
\begin{aligned}
    E(\overline X^2 - cS^2)&=E(\overline X^2)-cE(S^2) = (\frac{\sigma^2}{n}+\mu^2)-c\sigma^2=\mu^2
\end{aligned}
\]

故，

\[
    c = \frac{1}{n}
\]

### 13. 解：

#### (1)

由题知，$E(\hat\theta)=\theta, D(\hat\theta) > 0, \hat\theta^2=(\hat\theta)^2$

故，

\[
    E(\hat\theta^2) = E((\hat\theta)^2)=D(\hat\theta)+E(\hat\theta)^2=D(\hat\theta) + \theta^2>\theta^2
\]

#### (2)

似然函数为，

\[
\begin{aligned}
    L(\theta) = 
    \begin{cases}
        \frac{1}{\theta^n} & 0 < x_1,x_2,...,x_n \le \theta \\
        0 & \rm otherwise
    \end{cases}
\end{aligned}
\]

故最大似然估计量 \( \hat\theta \) 为，

\[
    \hat\theta = \max\{x_1,x_2,...,x_n\}
\]

总体 \( X \) 分布函数为，

\[
    F(X)=
    \begin{cases}
        0 & x < 0 \\
        \frac{x}{\theta} & 0 \le x < \theta \\
        1 & x \ge \theta
    \end{cases}    
\]

故，

\[
\begin{aligned}
    F_{\hat\theta}(x) = F_{\rm max}(x) = (F(x)) ^ n = 
    \begin{cases}
        0 & x < 0 \\
        (\frac{x}{\theta}) ^ n & 0\le x < \theta \\
        1 & x \ge \theta
    \end{cases}
\end{aligned}
\]

故，

\[
    f_{\hat\theta}(x)=
    \begin{cases}
        \frac{n}{\theta}(\frac{x}{\theta})^{n - 1} & 0\le z \le \theta \\
        0 & \rm otherwise
    \end{cases}    
\]

故，

\[
    E(\hat\theta) = \int_{-\infty}^{+\infty} xf_{\hat\theta}(x) {\rm d} x = \int_0^\theta n(\frac{x}{\theta}) ^ n{\rm d} x=\frac{n\theta}{n + 1} \neq \theta
\]

### 15. 解：

\[
    E(\hat\theta) = E(\sum\limits_{i = 1}^na_iX_i)=\sum\limits_{i=1}^na_iE(X_i)=\theta\sum\limits_{i=1}^na_i
\]

故有，

\[
    \sum\limits_{i=1}^na_i = 1
\]

\[
\begin{aligned}
    D(\hat\theta) &= \sum\limits_{i=1}^n a_i^2D(X_i)=\sum\limits_{i=1}^na_i^2\sigma_i^2
\end{aligned}
\]

作函数

\[
    g(a_1, a_2, ..., a_n, \lambda) = \sum\limits_{i=1}^na_i^2\sigma_i^2 + \lambda(\sum\limits_{i = 1} ^ n a_i-1)
\]

令

\[
    \frac{\partial g}{\partial a_i} = 2\sigma_i^2 a_i + \lambda = 0  \\
    \frac{\partial g}{\partial \lambda} = \sum\limits_{i=1}^n a_i-1 = 0
\]

故有 \( a_i=-\frac{\lambda}{2\sigma_i^2} \)，代入得，

\[
    -\frac{\lambda}{2}\sum\limits_{i=1}^n\frac{1}{\sigma_i^2}=1
\]

故，

\[
    \lambda = -\frac{2}{\sum_{i=1}^n\frac{1}{\sigma_i^2}} \\
    a_i=\frac{1}{\sigma_i^2\sum_{j=1}^n\frac{1}{\sigma_j^2}}
\]