### 9. 解：

$$
f(x,y)=
\begin{cases}
    cx^2y & x^2 \leq y \leq 1 \\
    0 & \rm otherwise
\end{cases}
$$

#### （1）

由题意知，

$$
\begin{aligned}
    \iint\limits_{D} f(x,y) dxdy &= \int_{-1}^1\int_{x^2}^1 cx^2ydxdy\\
    &= c\int_{-1}^1x^2\cdot\frac{1}{2}(1 - x^4)dx\\
    &=\frac{4c}{21}\\
    &=1
\end{aligned}
$$

故，$c=\frac{21}{4}$

#### （2）

$$
\begin{aligned}
f_X(x)&=\frac{21}{4}\int_{x^2}^1x^2ydy=\frac{21}{8}(x^2-x^6) \\
f_Y(y)&=\frac{21}{4}\int_{-\sqrt y}^{\sqrt y} x^2ydx=\frac{7}{2}y^{\frac{3}{2}}
\end{aligned}
$$

故，

$$
\begin{aligned}
    f_X(x) &= 
    \begin{cases}
        \frac{21}{8}(x^2-x^6) & |x|\leq 1 \\
        0 & \rm otherwise
    \end{cases}\\
    f_Y(y) &= 
    \begin{cases}
        \frac{7}{2}y^{\frac{3}{2}} & 0\leq y\leq 1 \\
        0 & \rm otherwise
    \end{cases}
\end{aligned}
$$

#### 11. 解：

#### （1）

$$
\begin{aligned}
    f_X(x)&=\sum\limits_{y=0}^x\frac{e^{-14}7.14^y6.86^{x-y}}{y!(x-y)!} \\
    &= \frac{e^{-14}}{x!}\sum\limits_{y=0}^x\binom{x}{y}7.14^y6.86^{x-y}\\
    &= \frac{e^{-14}}{x!}(7.14+6.86)^x \\
    &= \frac{14^xe^{-14}}{x!}\\
    f_Y(y) &= \sum\limits_{x=y}^\infty\frac{e^{-14}7.14^y6.86^{x-y}}{y!(x-y)!}\\
    &= \sum\limits_{x=0}^\infty \frac{e^{-14}7.14^y6.86^x}{y!x!}\\
    &=\frac{7.14^ye^{-14}}{y!}\sum\limits_{x=0}^\infty \frac{6.86^x}{x!} \\
    &= \frac{7.14^ye^{-14}}{y!}\cdot e^{6.86}\\
    &= \frac{7.14^y}{e^{7.14}y!}
\end{aligned}
$$